Isabelle/AList_ext.thy
@@ -41,7 +41,7 @@ by (induct l) (auto simp add: lookup_def)
 lemma alist_keys_fst_set[simp]: "keys l = fst ` set l"
 by (induct l) (auto simp add: keys_def)
 
-(* TODO: improve speed! *)
+(* TODO: improve proof speed! *)
 lemma alist_partition_distr: "is_alist l \<Longrightarrow> (yes, no) = partition P l \<Longrightarrow> is_alist (yes @ no)"
 unfolding is_alist_def apply (induct l arbitrary: yes no) by auto
 
